Added Autosubst

syntax.sig
@@ -1,0 +1,19 @@
+lvl : Type
+ty : Type
+term(var_term) : Type
+russ_term(r_var_term) : Type
+
+Prod : ty -> (bind term in ty) -> ty
+Decode : lvl -> term -> ty
+U : lvl -> ty
+
+Lambda : ty -> (bind term in ty) -> (bind term in term) -> term
+App : ty -> (bind term in ty) -> term -> term -> term
+cProd : lvl -> term -> (bind term in term) -> term
+cU : lvl -> lvl -> term
+cLift : lvl -> lvl -> term -> term
+
+r_Prod : russ_term -> (bind russ_term in russ_term) -> russ_term
+r_U : lvl -> russ_term
+r_Lambda : russ_term -> (bind russ_term in russ_term) -> (bind russ_term in russ_term) -> russ_term
+r_App : russ_term -> (bind russ_term in russ_term) -> russ_term -> russ_term -> russ_term
