Autosubst.v
@@ -1,0 +1,1803 @@
+Require Import RussellTarskiEquivalence.core.
+Require Import RussellTarskiEquivalence.unscoped.
+
+Require Import Setoid Morphisms Relation_Definitions.
+Module Core.
+
+Definition lvl := nat.
+
+Inductive russ_term : Type :=
+  | r_var_term : nat -> russ_term
+  | r_Prod : russ_term -> russ_term -> russ_term
+  | r_U : lvl -> russ_term
+  | r_Lambda : russ_term -> russ_term -> russ_term -> russ_term
+  | r_App : russ_term -> russ_term -> russ_term -> russ_term -> russ_term.
+
+Lemma congr_r_Prod {s0 : russ_term} {s1 : russ_term} {t0 : russ_term}
+  {t1 : russ_term} (H0 : s0 = t0) (H1 : s1 = t1) :
+  r_Prod s0 s1 = r_Prod t0 t1.
+Proof.
+exact (eq_trans (eq_trans eq_refl (ap (fun x => r_Prod x s1) H0))
+         (ap (fun x => r_Prod t0 x) H1)).
+Qed.
+
+Lemma congr_r_U {s0 : lvl} {t0 : lvl} (H0 : s0 = t0) : r_U s0 = r_U t0.
+Proof.
+exact (eq_trans eq_refl (ap (fun x => r_U x) H0)).
+Qed.
+
+Lemma congr_r_Lambda {s0 : russ_term} {s1 : russ_term} {s2 : russ_term}
+  {t0 : russ_term} {t1 : russ_term} {t2 : russ_term} (H0 : s0 = t0)
+  (H1 : s1 = t1) (H2 : s2 = t2) : r_Lambda s0 s1 s2 = r_Lambda t0 t1 t2.
+Proof.
+exact (eq_trans
+         (eq_trans (eq_trans eq_refl (ap (fun x => r_Lambda x s1 s2) H0))
+            (ap (fun x => r_Lambda t0 x s2) H1))
+         (ap (fun x => r_Lambda t0 t1 x) H2)).
+Qed.
+
+Lemma congr_r_App {s0 : russ_term} {s1 : russ_term} {s2 : russ_term}
+  {s3 : russ_term} {t0 : russ_term} {t1 : russ_term} {t2 : russ_term}
+  {t3 : russ_term} (H0 : s0 = t0) (H1 : s1 = t1) (H2 : s2 = t2)
+  (H3 : s3 = t3) : r_App s0 s1 s2 s3 = r_App t0 t1 t2 t3.
+Proof.
+exact (eq_trans
+         (eq_trans
+            (eq_trans (eq_trans eq_refl (ap (fun x => r_App x s1 s2 s3) H0))
+               (ap (fun x => r_App t0 x s2 s3) H1))
+            (ap (fun x => r_App t0 t1 x s3) H2))
+         (ap (fun x => r_App t0 t1 t2 x) H3)).
+Qed.
+
+Lemma upRen_russ_term_russ_term (xi : nat -> nat) : nat -> nat.
+Proof.
+exact (up_ren xi).
+Defined.
+
+Fixpoint ren_russ_term (xi_russ_term : nat -> nat) (s : russ_term) {struct s}
+   : russ_term :=
+  match s with
+  | r_var_term s0 => r_var_term (xi_russ_term s0)
+  | r_Prod s0 s1 =>
+      r_Prod (ren_russ_term xi_russ_term s0)
+        (ren_russ_term (upRen_russ_term_russ_term xi_russ_term) s1)
+  | r_U s0 => r_U s0
+  | r_Lambda s0 s1 s2 =>
+      r_Lambda (ren_russ_term xi_russ_term s0)
+        (ren_russ_term (upRen_russ_term_russ_term xi_russ_term) s1)
+        (ren_russ_term (upRen_russ_term_russ_term xi_russ_term) s2)
+  | r_App s0 s1 s2 s3 =>
+      r_App (ren_russ_term xi_russ_term s0)
+        (ren_russ_term (upRen_russ_term_russ_term xi_russ_term) s1)
+        (ren_russ_term xi_russ_term s2) (ren_russ_term xi_russ_term s3)
+  end.
+
+Lemma up_russ_term_russ_term (sigma : nat -> russ_term) : nat -> russ_term.
+Proof.
+exact (scons (r_var_term var_zero) (funcomp (ren_russ_term shift) sigma)).
+Defined.
+
+Fixpoint subst_russ_term (sigma_russ_term : nat -> russ_term) (s : russ_term)
+{struct s} : russ_term :=
+  match s with
+  | r_var_term s0 => sigma_russ_term s0
+  | r_Prod s0 s1 =>
+      r_Prod (subst_russ_term sigma_russ_term s0)
+        (subst_russ_term (up_russ_term_russ_term sigma_russ_term) s1)
+  | r_U s0 => r_U s0
+  | r_Lambda s0 s1 s2 =>
+      r_Lambda (subst_russ_term sigma_russ_term s0)
+        (subst_russ_term (up_russ_term_russ_term sigma_russ_term) s1)
+        (subst_russ_term (up_russ_term_russ_term sigma_russ_term) s2)
+  | r_App s0 s1 s2 s3 =>
+      r_App (subst_russ_term sigma_russ_term s0)
+        (subst_russ_term (up_russ_term_russ_term sigma_russ_term) s1)
+        (subst_russ_term sigma_russ_term s2)
+        (subst_russ_term sigma_russ_term s3)
+  end.
+
+Lemma upId_russ_term_russ_term (sigma : nat -> russ_term)
+  (Eq : forall x, sigma x = r_var_term x) :
+  forall x, up_russ_term_russ_term sigma x = r_var_term x.
+Proof.
+exact (fun n =>
+       match n with
+       | S n' => ap (ren_russ_term shift) (Eq n')
+       | O => eq_refl
+       end).
+Qed.
+
+Fixpoint idSubst_russ_term (sigma_russ_term : nat -> russ_term)
+(Eq_russ_term : forall x, sigma_russ_term x = r_var_term x) (s : russ_term)
+{struct s} : subst_russ_term sigma_russ_term s = s :=
+  match s with
+  | r_var_term s0 => Eq_russ_term s0
+  | r_Prod s0 s1 =>
+      congr_r_Prod (idSubst_russ_term sigma_russ_term Eq_russ_term s0)
+        (idSubst_russ_term (up_russ_term_russ_term sigma_russ_term)
+           (upId_russ_term_russ_term _ Eq_russ_term) s1)
+  | r_U s0 => congr_r_U (eq_refl s0)
+  | r_Lambda s0 s1 s2 =>
+      congr_r_Lambda (idSubst_russ_term sigma_russ_term Eq_russ_term s0)
+        (idSubst_russ_term (up_russ_term_russ_term sigma_russ_term)
+           (upId_russ_term_russ_term _ Eq_russ_term) s1)
+        (idSubst_russ_term (up_russ_term_russ_term sigma_russ_term)
+           (upId_russ_term_russ_term _ Eq_russ_term) s2)
+  | r_App s0 s1 s2 s3 =>
+      congr_r_App (idSubst_russ_term sigma_russ_term Eq_russ_term s0)
+        (idSubst_russ_term (up_russ_term_russ_term sigma_russ_term)
+           (upId_russ_term_russ_term _ Eq_russ_term) s1)
+        (idSubst_russ_term sigma_russ_term Eq_russ_term s2)
+        (idSubst_russ_term sigma_russ_term Eq_russ_term s3)
+  end.
+
+Lemma upExtRen_russ_term_russ_term (xi : nat -> nat) (zeta : nat -> nat)
+  (Eq : forall x, xi x = zeta x) :
+  forall x, upRen_russ_term_russ_term xi x = upRen_russ_term_russ_term zeta x.
+Proof.
+exact (fun n => match n with
+                | S n' => ap shift (Eq n')
+                | O => eq_refl
+                end).
+Qed.
+
+Fixpoint extRen_russ_term (xi_russ_term : nat -> nat)
+(zeta_russ_term : nat -> nat)
+(Eq_russ_term : forall x, xi_russ_term x = zeta_russ_term x) (s : russ_term)
+{struct s} : ren_russ_term xi_russ_term s = ren_russ_term zeta_russ_term s :=
+  match s with
+  | r_var_term s0 => ap (r_var_term) (Eq_russ_term s0)
+  | r_Prod s0 s1 =>
+      congr_r_Prod
+        (extRen_russ_term xi_russ_term zeta_russ_term Eq_russ_term s0)
+        (extRen_russ_term (upRen_russ_term_russ_term xi_russ_term)
+           (upRen_russ_term_russ_term zeta_russ_term)
+           (upExtRen_russ_term_russ_term _ _ Eq_russ_term) s1)
+  | r_U s0 => congr_r_U (eq_refl s0)
+  | r_Lambda s0 s1 s2 =>
+      congr_r_Lambda
+        (extRen_russ_term xi_russ_term zeta_russ_term Eq_russ_term s0)
+        (extRen_russ_term (upRen_russ_term_russ_term xi_russ_term)
+           (upRen_russ_term_russ_term zeta_russ_term)
+           (upExtRen_russ_term_russ_term _ _ Eq_russ_term) s1)
+        (extRen_russ_term (upRen_russ_term_russ_term xi_russ_term)
+           (upRen_russ_term_russ_term zeta_russ_term)
+           (upExtRen_russ_term_russ_term _ _ Eq_russ_term) s2)
+  | r_App s0 s1 s2 s3 =>
+      congr_r_App
+        (extRen_russ_term xi_russ_term zeta_russ_term Eq_russ_term s0)
+        (extRen_russ_term (upRen_russ_term_russ_term xi_russ_term)
+           (upRen_russ_term_russ_term zeta_russ_term)
+           (upExtRen_russ_term_russ_term _ _ Eq_russ_term) s1)
+        (extRen_russ_term xi_russ_term zeta_russ_term Eq_russ_term s2)
+        (extRen_russ_term xi_russ_term zeta_russ_term Eq_russ_term s3)
+  end.
+
+Lemma upExt_russ_term_russ_term (sigma : nat -> russ_term)
+  (tau : nat -> russ_term) (Eq : forall x, sigma x = tau x) :
+  forall x, up_russ_term_russ_term sigma x = up_russ_term_russ_term tau x.
+Proof.
+exact (fun n =>
+       match n with
+       | S n' => ap (ren_russ_term shift) (Eq n')
+       | O => eq_refl
+       end).
+Qed.
+
+Fixpoint ext_russ_term (sigma_russ_term : nat -> russ_term)
+(tau_russ_term : nat -> russ_term)
+(Eq_russ_term : forall x, sigma_russ_term x = tau_russ_term x)
+(s : russ_term) {struct s} :
+subst_russ_term sigma_russ_term s = subst_russ_term tau_russ_term s :=
+  match s with
+  | r_var_term s0 => Eq_russ_term s0
+  | r_Prod s0 s1 =>
+      congr_r_Prod
+        (ext_russ_term sigma_russ_term tau_russ_term Eq_russ_term s0)
+        (ext_russ_term (up_russ_term_russ_term sigma_russ_term)
+           (up_russ_term_russ_term tau_russ_term)
+           (upExt_russ_term_russ_term _ _ Eq_russ_term) s1)
+  | r_U s0 => congr_r_U (eq_refl s0)
+  | r_Lambda s0 s1 s2 =>
+      congr_r_Lambda
+        (ext_russ_term sigma_russ_term tau_russ_term Eq_russ_term s0)
+        (ext_russ_term (up_russ_term_russ_term sigma_russ_term)
+           (up_russ_term_russ_term tau_russ_term)
+           (upExt_russ_term_russ_term _ _ Eq_russ_term) s1)
+        (ext_russ_term (up_russ_term_russ_term sigma_russ_term)
+           (up_russ_term_russ_term tau_russ_term)
+           (upExt_russ_term_russ_term _ _ Eq_russ_term) s2)
+  | r_App s0 s1 s2 s3 =>
+      congr_r_App
+        (ext_russ_term sigma_russ_term tau_russ_term Eq_russ_term s0)
+        (ext_russ_term (up_russ_term_russ_term sigma_russ_term)
+           (up_russ_term_russ_term tau_russ_term)
+           (upExt_russ_term_russ_term _ _ Eq_russ_term) s1)
+        (ext_russ_term sigma_russ_term tau_russ_term Eq_russ_term s2)
+        (ext_russ_term sigma_russ_term tau_russ_term Eq_russ_term s3)
+  end.
+  
+
+Lemma up_ren_ren_russ_term_russ_term (xi : nat -> nat) (zeta : nat -> nat)
+  (rho : nat -> nat) (Eq : forall x, funcomp zeta xi x = rho x) :
+  forall x,
+  funcomp (upRen_russ_term_russ_term zeta) (upRen_russ_term_russ_term xi) x =
+  upRen_russ_term_russ_term rho x.
+Proof.
+exact (up_ren_ren xi zeta rho Eq).
+Qed.
+
+Fixpoint compRenRen_russ_term (xi_russ_term : nat -> nat)
+(zeta_russ_term : nat -> nat) (rho_russ_term : nat -> nat)
+(Eq_russ_term : forall x,
+                funcomp zeta_russ_term xi_russ_term x = rho_russ_term x)
+(s : russ_term) {struct s} :
+ren_russ_term zeta_russ_term (ren_russ_term xi_russ_term s) =
+ren_russ_term rho_russ_term s :=
+  match s with
+  | r_var_term s0 => ap (r_var_term) (Eq_russ_term s0)
+  | r_Prod s0 s1 =>
+      congr_r_Prod
+        (compRenRen_russ_term xi_russ_term zeta_russ_term rho_russ_term
+           Eq_russ_term s0)
+        (compRenRen_russ_term (upRen_russ_term_russ_term xi_russ_term)
+           (upRen_russ_term_russ_term zeta_russ_term)
+           (upRen_russ_term_russ_term rho_russ_term)
+           (up_ren_ren _ _ _ Eq_russ_term) s1)
+  | r_U s0 => congr_r_U (eq_refl s0)
+  | r_Lambda s0 s1 s2 =>
+      congr_r_Lambda
+        (compRenRen_russ_term xi_russ_term zeta_russ_term rho_russ_term
+           Eq_russ_term s0)
+        (compRenRen_russ_term (upRen_russ_term_russ_term xi_russ_term)
+           (upRen_russ_term_russ_term zeta_russ_term)
+           (upRen_russ_term_russ_term rho_russ_term)
+           (up_ren_ren _ _ _ Eq_russ_term) s1)
+        (compRenRen_russ_term (upRen_russ_term_russ_term xi_russ_term)
+           (upRen_russ_term_russ_term zeta_russ_term)
+           (upRen_russ_term_russ_term rho_russ_term)
+           (up_ren_ren _ _ _ Eq_russ_term) s2)
+  | r_App s0 s1 s2 s3 =>
+      congr_r_App
+        (compRenRen_russ_term xi_russ_term zeta_russ_term rho_russ_term
+           Eq_russ_term s0)
+        (compRenRen_russ_term (upRen_russ_term_russ_term xi_russ_term)
+           (upRen_russ_term_russ_term zeta_russ_term)
+           (upRen_russ_term_russ_term rho_russ_term)
+           (up_ren_ren _ _ _ Eq_russ_term) s1)
+        (compRenRen_russ_term xi_russ_term zeta_russ_term rho_russ_term
+           Eq_russ_term s2)
+        (compRenRen_russ_term xi_russ_term zeta_russ_term rho_russ_term
+           Eq_russ_term s3)
+  end.
+
+Lemma up_ren_subst_russ_term_russ_term (xi : nat -> nat)
+  (tau : nat -> russ_term) (theta : nat -> russ_term)
+  (Eq : forall x, funcomp tau xi x = theta x) :
+  forall x,
+  funcomp (up_russ_term_russ_term tau) (upRen_russ_term_russ_term xi) x =
+  up_russ_term_russ_term theta x.
+Proof.
+exact (fun n =>
+       match n with
+       | S n' => ap (ren_russ_term shift) (Eq n')
+       | O => eq_refl
+       end).
+Qed.
+
+Fixpoint compRenSubst_russ_term (xi_russ_term : nat -> nat)
+(tau_russ_term : nat -> russ_term) (theta_russ_term : nat -> russ_term)
+(Eq_russ_term : forall x,
+                funcomp tau_russ_term xi_russ_term x = theta_russ_term x)
+(s : russ_term) {struct s} :
+subst_russ_term tau_russ_term (ren_russ_term xi_russ_term s) =
+subst_russ_term theta_russ_term s :=
+  match s with
+  | r_var_term s0 => Eq_russ_term s0
+  | r_Prod s0 s1 =>
+      congr_r_Prod
+        (compRenSubst_russ_term xi_russ_term tau_russ_term theta_russ_term
+           Eq_russ_term s0)
+        (compRenSubst_russ_term (upRen_russ_term_russ_term xi_russ_term)
+           (up_russ_term_russ_term tau_russ_term)
+           (up_russ_term_russ_term theta_russ_term)
+           (up_ren_subst_russ_term_russ_term _ _ _ Eq_russ_term) s1)
+  | r_U s0 => congr_r_U (eq_refl s0)
+  | r_Lambda s0 s1 s2 =>
+      congr_r_Lambda
+        (compRenSubst_russ_term xi_russ_term tau_russ_term theta_russ_term
+           Eq_russ_term s0)
+        (compRenSubst_russ_term (upRen_russ_term_russ_term xi_russ_term)
+           (up_russ_term_russ_term tau_russ_term)
+           (up_russ_term_russ_term theta_russ_term)
+           (up_ren_subst_russ_term_russ_term _ _ _ Eq_russ_term) s1)
+        (compRenSubst_russ_term (upRen_russ_term_russ_term xi_russ_term)
+           (up_russ_term_russ_term tau_russ_term)
+           (up_russ_term_russ_term theta_russ_term)
+           (up_ren_subst_russ_term_russ_term _ _ _ Eq_russ_term) s2)
+  | r_App s0 s1 s2 s3 =>
+      congr_r_App
+        (compRenSubst_russ_term xi_russ_term tau_russ_term theta_russ_term
+           Eq_russ_term s0)
+        (compRenSubst_russ_term (upRen_russ_term_russ_term xi_russ_term)
+           (up_russ_term_russ_term tau_russ_term)
+           (up_russ_term_russ_term theta_russ_term)
+           (up_ren_subst_russ_term_russ_term _ _ _ Eq_russ_term) s1)
+        (compRenSubst_russ_term xi_russ_term tau_russ_term theta_russ_term
+           Eq_russ_term s2)
+        (compRenSubst_russ_term xi_russ_term tau_russ_term theta_russ_term
+           Eq_russ_term s3)
+  end.
+
+Lemma up_subst_ren_russ_term_russ_term (sigma : nat -> russ_term)
+  (zeta_russ_term : nat -> nat) (theta : nat -> russ_term)
+  (Eq : forall x, funcomp (ren_russ_term zeta_russ_term) sigma x = theta x) :
+  forall x,
+  funcomp (ren_russ_term (upRen_russ_term_russ_term zeta_russ_term))
+    (up_russ_term_russ_term sigma) x = up_russ_term_russ_term theta x.
+Proof.
+exact (fun n =>
+       match n with
+       | S n' =>
+           eq_trans
+             (compRenRen_russ_term shift
+                (upRen_russ_term_russ_term zeta_russ_term)
+                (funcomp shift zeta_russ_term) (fun x => eq_refl) (sigma n'))
+             (eq_trans
+                (eq_sym
+                   (compRenRen_russ_term zeta_russ_term shift
+                      (funcomp shift zeta_russ_term) (fun x => eq_refl)
+                      (sigma n'))) (ap (ren_russ_term shift) (Eq n')))
+       | O => eq_refl
+       end).
+Qed.
+
+Fixpoint compSubstRen_russ_term (sigma_russ_term : nat -> russ_term)
+(zeta_russ_term : nat -> nat) (theta_russ_term : nat -> russ_term)
+(Eq_russ_term : forall x,
+                funcomp (ren_russ_term zeta_russ_term) sigma_russ_term x =
+                theta_russ_term x) (s : russ_term) {struct s} :
+ren_russ_term zeta_russ_term (subst_russ_term sigma_russ_term s) =
+subst_russ_term theta_russ_term s :=
+  match s with
+  | r_var_term s0 => Eq_russ_term s0
+  | r_Prod s0 s1 =>
+      congr_r_Prod
+        (compSubstRen_russ_term sigma_russ_term zeta_russ_term
+           theta_russ_term Eq_russ_term s0)
+        (compSubstRen_russ_term (up_russ_term_russ_term sigma_russ_term)
+           (upRen_russ_term_russ_term zeta_russ_term)
+           (up_russ_term_russ_term theta_russ_term)
+           (up_subst_ren_russ_term_russ_term _ _ _ Eq_russ_term) s1)
+  | r_U s0 => congr_r_U (eq_refl s0)
+  | r_Lambda s0 s1 s2 =>
+      congr_r_Lambda
+        (compSubstRen_russ_term sigma_russ_term zeta_russ_term
+           theta_russ_term Eq_russ_term s0)
+        (compSubstRen_russ_term (up_russ_term_russ_term sigma_russ_term)
+           (upRen_russ_term_russ_term zeta_russ_term)
+           (up_russ_term_russ_term theta_russ_term)
+           (up_subst_ren_russ_term_russ_term _ _ _ Eq_russ_term) s1)
+        (compSubstRen_russ_term (up_russ_term_russ_term sigma_russ_term)
+           (upRen_russ_term_russ_term zeta_russ_term)
+           (up_russ_term_russ_term theta_russ_term)
+           (up_subst_ren_russ_term_russ_term _ _ _ Eq_russ_term) s2)
+  | r_App s0 s1 s2 s3 =>
+      congr_r_App
+        (compSubstRen_russ_term sigma_russ_term zeta_russ_term
+           theta_russ_term Eq_russ_term s0)
+        (compSubstRen_russ_term (up_russ_term_russ_term sigma_russ_term)
+           (upRen_russ_term_russ_term zeta_russ_term)
+           (up_russ_term_russ_term theta_russ_term)
+           (up_subst_ren_russ_term_russ_term _ _ _ Eq_russ_term) s1)
+        (compSubstRen_russ_term sigma_russ_term zeta_russ_term
+           theta_russ_term Eq_russ_term s2)
+        (compSubstRen_russ_term sigma_russ_term zeta_russ_term
+           theta_russ_term Eq_russ_term s3)
+  end.
+
+Lemma up_subst_subst_russ_term_russ_term (sigma : nat -> russ_term)
+  (tau_russ_term : nat -> russ_term) (theta : nat -> russ_term)
+  (Eq : forall x, funcomp (subst_russ_term tau_russ_term) sigma x = theta x)
+  :
+  forall x,
+  funcomp (subst_russ_term (up_russ_term_russ_term tau_russ_term))
+    (up_russ_term_russ_term sigma) x = up_russ_term_russ_term theta x.
+Proof.
+exact (fun n =>
+       match n with
+       | S n' =>
+           eq_trans
+             (compRenSubst_russ_term shift
+                (up_russ_term_russ_term tau_russ_term)
+                (funcomp (up_russ_term_russ_term tau_russ_term) shift)
+                (fun x => eq_refl) (sigma n'))
+             (eq_trans
+                (eq_sym
+                   (compSubstRen_russ_term tau_russ_term shift
+                      (funcomp (ren_russ_term shift) tau_russ_term)
+                      (fun x => eq_refl) (sigma n')))
+                (ap (ren_russ_term shift) (Eq n')))
+       | O => eq_refl
+       end).
+Qed.
+
+Fixpoint compSubstSubst_russ_term (sigma_russ_term : nat -> russ_term)
+(tau_russ_term : nat -> russ_term) (theta_russ_term : nat -> russ_term)
+(Eq_russ_term : forall x,
+                funcomp (subst_russ_term tau_russ_term) sigma_russ_term x =
+                theta_russ_term x) (s : russ_term) {struct s} :
+subst_russ_term tau_russ_term (subst_russ_term sigma_russ_term s) =
+subst_russ_term theta_russ_term s :=
+  match s with
+  | r_var_term s0 => Eq_russ_term s0
+  | r_Prod s0 s1 =>
+      congr_r_Prod
+        (compSubstSubst_russ_term sigma_russ_term tau_russ_term
+           theta_russ_term Eq_russ_term s0)
+        (compSubstSubst_russ_term (up_russ_term_russ_term sigma_russ_term)
+           (up_russ_term_russ_term tau_russ_term)
+           (up_russ_term_russ_term theta_russ_term)
+           (up_subst_subst_russ_term_russ_term _ _ _ Eq_russ_term) s1)
+  | r_U s0 => congr_r_U (eq_refl s0)
+  | r_Lambda s0 s1 s2 =>
+      congr_r_Lambda
+        (compSubstSubst_russ_term sigma_russ_term tau_russ_term
+           theta_russ_term Eq_russ_term s0)
+        (compSubstSubst_russ_term (up_russ_term_russ_term sigma_russ_term)
+           (up_russ_term_russ_term tau_russ_term)
+           (up_russ_term_russ_term theta_russ_term)
+           (up_subst_subst_russ_term_russ_term _ _ _ Eq_russ_term) s1)
+        (compSubstSubst_russ_term (up_russ_term_russ_term sigma_russ_term)
+           (up_russ_term_russ_term tau_russ_term)
+           (up_russ_term_russ_term theta_russ_term)
+           (up_subst_subst_russ_term_russ_term _ _ _ Eq_russ_term) s2)
+  | r_App s0 s1 s2 s3 =>
+      congr_r_App
+        (compSubstSubst_russ_term sigma_russ_term tau_russ_term
+           theta_russ_term Eq_russ_term s0)
+        (compSubstSubst_russ_term (up_russ_term_russ_term sigma_russ_term)
+           (up_russ_term_russ_term tau_russ_term)
+           (up_russ_term_russ_term theta_russ_term)
+           (up_subst_subst_russ_term_russ_term _ _ _ Eq_russ_term) s1)
+        (compSubstSubst_russ_term sigma_russ_term tau_russ_term
+           theta_russ_term Eq_russ_term s2)
+        (compSubstSubst_russ_term sigma_russ_term tau_russ_term
+           theta_russ_term Eq_russ_term s3)
+  end.
+
+Lemma renRen_russ_term (xi_russ_term : nat -> nat)
+  (zeta_russ_term : nat -> nat) (s : russ_term) :
+  ren_russ_term zeta_russ_term (ren_russ_term xi_russ_term s) =
+  ren_russ_term (funcomp zeta_russ_term xi_russ_term) s.
+Proof.
+exact (compRenRen_russ_term xi_russ_term zeta_russ_term _ (fun n => eq_refl)
+         s).
+Qed.
+
+Lemma renRen'_russ_term_pointwise (xi_russ_term : nat -> nat)
+  (zeta_russ_term : nat -> nat) :
+  pointwise_relation _ eq
+    (funcomp (ren_russ_term zeta_russ_term) (ren_russ_term xi_russ_term))
+    (ren_russ_term (funcomp zeta_russ_term xi_russ_term)).
+Proof.
+exact (fun s =>
+       compRenRen_russ_term xi_russ_term zeta_russ_term _ (fun n => eq_refl)
+         s).
+Qed.
+
+Lemma renSubst_russ_term (xi_russ_term : nat -> nat)
+  (tau_russ_term : nat -> russ_term) (s : russ_term) :
+  subst_russ_term tau_russ_term (ren_russ_term xi_russ_term s) =
+  subst_russ_term (funcomp tau_russ_term xi_russ_term) s.
+Proof.
+exact (compRenSubst_russ_term xi_russ_term tau_russ_term _ (fun n => eq_refl)
+         s).
+Qed.
+
+Lemma renSubst_russ_term_pointwise (xi_russ_term : nat -> nat)
+  (tau_russ_term : nat -> russ_term) :
+  pointwise_relation _ eq
+    (funcomp (subst_russ_term tau_russ_term) (ren_russ_term xi_russ_term))
+    (subst_russ_term (funcomp tau_russ_term xi_russ_term)).
+Proof.
+exact (fun s =>
+       compRenSubst_russ_term xi_russ_term tau_russ_term _ (fun n => eq_refl)
+         s).
+Qed.
+
+Lemma substRen_russ_term (sigma_russ_term : nat -> russ_term)
+  (zeta_russ_term : nat -> nat) (s : russ_term) :
+  ren_russ_term zeta_russ_term (subst_russ_term sigma_russ_term s) =
+  subst_russ_term (funcomp (ren_russ_term zeta_russ_term) sigma_russ_term) s.
+Proof.
+exact (compSubstRen_russ_term sigma_russ_term zeta_russ_term _
+         (fun n => eq_refl) s).
+Qed.
+
+Lemma substRen_russ_term_pointwise (sigma_russ_term : nat -> russ_term)
+  (zeta_russ_term : nat -> nat) :
+  pointwise_relation _ eq
+    (funcomp (ren_russ_term zeta_russ_term) (subst_russ_term sigma_russ_term))
+    (subst_russ_term (funcomp (ren_russ_term zeta_russ_term) sigma_russ_term)).
+Proof.
+exact (fun s =>
+       compSubstRen_russ_term sigma_russ_term zeta_russ_term _
+         (fun n => eq_refl) s).
+Qed.
+
+Lemma substSubst_russ_term (sigma_russ_term : nat -> russ_term)
+  (tau_russ_term : nat -> russ_term) (s : russ_term) :
+  subst_russ_term tau_russ_term (subst_russ_term sigma_russ_term s) =
+  subst_russ_term (funcomp (subst_russ_term tau_russ_term) sigma_russ_term) s.
+Proof.
+exact (compSubstSubst_russ_term sigma_russ_term tau_russ_term _
+         (fun n => eq_refl) s).
+Qed.
+
+Lemma substSubst_russ_term_pointwise (sigma_russ_term : nat -> russ_term)
+  (tau_russ_term : nat -> russ_term) :
+  pointwise_relation _ eq
+    (funcomp (subst_russ_term tau_russ_term)
+       (subst_russ_term sigma_russ_term))
+    (subst_russ_term
+       (funcomp (subst_russ_term tau_russ_term) sigma_russ_term)).
+Proof.
+exact (fun s =>
+       compSubstSubst_russ_term sigma_russ_term tau_russ_term _
+         (fun n => eq_refl) s).
+Qed.
+
+Lemma rinstInst_up_russ_term_russ_term (xi : nat -> nat)
+  (sigma : nat -> russ_term)
+  (Eq : forall x, funcomp (r_var_term) xi x = sigma x) :
+  forall x,
+  funcomp (r_var_term) (upRen_russ_term_russ_term xi) x =
+  up_russ_term_russ_term sigma x.
+Proof.
+exact (fun n =>
+       match n with
+       | S n' => ap (ren_russ_term shift) (Eq n')
+       | O => eq_refl
+       end).
+Qed.
+
+Fixpoint rinst_inst_russ_term (xi_russ_term : nat -> nat)
+(sigma_russ_term : nat -> russ_term)
+(Eq_russ_term : forall x,
+                funcomp (r_var_term) xi_russ_term x = sigma_russ_term x)
+(s : russ_term) {struct s} :
+ren_russ_term xi_russ_term s = subst_russ_term sigma_russ_term s :=
+  match s with
+  | r_var_term s0 => Eq_russ_term s0
+  | r_Prod s0 s1 =>
+      congr_r_Prod
+        (rinst_inst_russ_term xi_russ_term sigma_russ_term Eq_russ_term s0)
+        (rinst_inst_russ_term (upRen_russ_term_russ_term xi_russ_term)
+           (up_russ_term_russ_term sigma_russ_term)
+           (rinstInst_up_russ_term_russ_term _ _ Eq_russ_term) s1)
+  | r_U s0 => congr_r_U (eq_refl s0)
+  | r_Lambda s0 s1 s2 =>
+      congr_r_Lambda
+        (rinst_inst_russ_term xi_russ_term sigma_russ_term Eq_russ_term s0)
+        (rinst_inst_russ_term (upRen_russ_term_russ_term xi_russ_term)
+           (up_russ_term_russ_term sigma_russ_term)
+           (rinstInst_up_russ_term_russ_term _ _ Eq_russ_term) s1)
+        (rinst_inst_russ_term (upRen_russ_term_russ_term xi_russ_term)
+           (up_russ_term_russ_term sigma_russ_term)
+           (rinstInst_up_russ_term_russ_term _ _ Eq_russ_term) s2)
+  | r_App s0 s1 s2 s3 =>
+      congr_r_App
+        (rinst_inst_russ_term xi_russ_term sigma_russ_term Eq_russ_term s0)
+        (rinst_inst_russ_term (upRen_russ_term_russ_term xi_russ_term)
+           (up_russ_term_russ_term sigma_russ_term)
+           (rinstInst_up_russ_term_russ_term _ _ Eq_russ_term) s1)
+        (rinst_inst_russ_term xi_russ_term sigma_russ_term Eq_russ_term s2)
+        (rinst_inst_russ_term xi_russ_term sigma_russ_term Eq_russ_term s3)
+  end.
+
+Lemma rinstInst'_russ_term (xi_russ_term : nat -> nat) (s : russ_term) :
+  ren_russ_term xi_russ_term s =
+  subst_russ_term (funcomp (r_var_term) xi_russ_term) s.
+Proof.
+exact (rinst_inst_russ_term xi_russ_term _ (fun n => eq_refl) s).
+Qed.
+
+Lemma rinstInst'_russ_term_pointwise (xi_russ_term : nat -> nat) :
+  pointwise_relation _ eq (ren_russ_term xi_russ_term)
+    (subst_russ_term (funcomp (r_var_term) xi_russ_term)).
+Proof.
+exact (fun s => rinst_inst_russ_term xi_russ_term _ (fun n => eq_refl) s).
+Qed.
+
+Lemma instId'_russ_term (s : russ_term) : subst_russ_term (r_var_term) s = s.
+Proof.
+exact (idSubst_russ_term (r_var_term) (fun n => eq_refl) s).
+Qed.
+
+Lemma instId'_russ_term_pointwise :
+  pointwise_relation _ eq (subst_russ_term (r_var_term)) id.
+Proof.
+exact (fun s => idSubst_russ_term (r_var_term) (fun n => eq_refl) s).
+Qed.
+
+Lemma rinstId'_russ_term (s : russ_term) : ren_russ_term id s = s.
+Proof.
+exact (eq_ind_r (fun t => t = s) (instId'_russ_term s)
+         (rinstInst'_russ_term id s)).
+Qed.
+
+Lemma rinstId'_russ_term_pointwise :
+  pointwise_relation _ eq (@ren_russ_term id) id.
+Proof.
+exact (fun s =>
+       eq_ind_r (fun t => t = s) (instId'_russ_term s)
+         (rinstInst'_russ_term id s)).
+Qed.
+
+Lemma varL'_russ_term (sigma_russ_term : nat -> russ_term) (x : nat) :
+  subst_russ_term sigma_russ_term (r_var_term x) = sigma_russ_term x.
+Proof.
+exact (eq_refl).
+Qed.
+
+Lemma varL'_russ_term_pointwise (sigma_russ_term : nat -> russ_term) :
+  pointwise_relation _ eq
+    (funcomp (subst_russ_term sigma_russ_term) (r_var_term)) sigma_russ_term.
+Proof.
+exact (fun x => eq_refl).
+Qed.
+
+Lemma varLRen'_russ_term (xi_russ_term : nat -> nat) (x : nat) :
+  ren_russ_term xi_russ_term (r_var_term x) = r_var_term (xi_russ_term x).
+Proof.
+exact (eq_refl).
+Qed.
+
+Lemma varLRen'_russ_term_pointwise (xi_russ_term : nat -> nat) :
+  pointwise_relation _ eq (funcomp (ren_russ_term xi_russ_term) (r_var_term))
+    (funcomp (r_var_term) xi_russ_term).
+Proof.
+exact (fun x => eq_refl).
+Qed.
+
+Inductive ty : Type :=
+  | Prod : ty -> ty -> ty
+  | Decode : lvl -> term -> ty
+  | U : lvl -> ty
+with term : Type :=
+  | var_term : nat -> term
+  | Lambda : ty -> ty -> term -> term
+  | App : ty -> ty -> term -> term -> term
+  | cProd : lvl -> term -> term -> term
+  | cU : lvl -> lvl -> term
+  | cLift : lvl -> lvl -> term -> term.
+
+Lemma congr_Prod {s0 : ty} {s1 : ty} {t0 : ty} {t1 : ty} (H0 : s0 = t0)
+  (H1 : s1 = t1) : Prod s0 s1 = Prod t0 t1.
+Proof.
+exact (eq_trans (eq_trans eq_refl (ap (fun x => Prod x s1) H0))
+         (ap (fun x => Prod t0 x) H1)).
+Qed.
+
+Lemma congr_Decode {s0 : lvl} {s1 : term} {t0 : lvl} {t1 : term}
+  (H0 : s0 = t0) (H1 : s1 = t1) : Decode s0 s1 = Decode t0 t1.
+Proof.
+exact (eq_trans (eq_trans eq_refl (ap (fun x => Decode x s1) H0))
+         (ap (fun x => Decode t0 x) H1)).
+Qed.
+
+Lemma congr_U {s0 : lvl} {t0 : lvl} (H0 : s0 = t0) : U s0 = U t0.
+Proof.
+exact (eq_trans eq_refl (ap (fun x => U x) H0)).
+Qed.
+
+Lemma congr_Lambda {s0 : ty} {s1 : ty} {s2 : term} {t0 : ty} {t1 : ty}
+  {t2 : term} (H0 : s0 = t0) (H1 : s1 = t1) (H2 : s2 = t2) :
+  Lambda s0 s1 s2 = Lambda t0 t1 t2.
+Proof.
+exact (eq_trans
+         (eq_trans (eq_trans eq_refl (ap (fun x => Lambda x s1 s2) H0))
+            (ap (fun x => Lambda t0 x s2) H1))
+         (ap (fun x => Lambda t0 t1 x) H2)).
+Qed.
+
+Lemma congr_App {s0 : ty} {s1 : ty} {s2 : term} {s3 : term} {t0 : ty}
+  {t1 : ty} {t2 : term} {t3 : term} (H0 : s0 = t0) (H1 : s1 = t1)
+  (H2 : s2 = t2) (H3 : s3 = t3) : App s0 s1 s2 s3 = App t0 t1 t2 t3.
+Proof.
+exact (eq_trans
+         (eq_trans
+            (eq_trans (eq_trans eq_refl (ap (fun x => App x s1 s2 s3) H0))
+               (ap (fun x => App t0 x s2 s3) H1))
+            (ap (fun x => App t0 t1 x s3) H2))
+         (ap (fun x => App t0 t1 t2 x) H3)).
+Qed.
+
+Lemma congr_cProd {s0 : lvl} {s1 : term} {s2 : term} {t0 : lvl} {t1 : term}
+  {t2 : term} (H0 : s0 = t0) (H1 : s1 = t1) (H2 : s2 = t2) :
+  cProd s0 s1 s2 = cProd t0 t1 t2.
+Proof.
+exact (eq_trans
+         (eq_trans (eq_trans eq_refl (ap (fun x => cProd x s1 s2) H0))
+            (ap (fun x => cProd t0 x s2) H1))
+         (ap (fun x => cProd t0 t1 x) H2)).
+Qed.
+
+Lemma congr_cU {s0 : lvl} {s1 : lvl} {t0 : lvl} {t1 : lvl} (H0 : s0 = t0)
+  (H1 : s1 = t1) : cU s0 s1 = cU t0 t1.
+Proof.
+exact (eq_trans (eq_trans eq_refl (ap (fun x => cU x s1) H0))
+         (ap (fun x => cU t0 x) H1)).
+Qed.
+
+Lemma congr_cLift {s0 : lvl} {s1 : lvl} {s2 : term} {t0 : lvl} {t1 : lvl}
+  {t2 : term} (H0 : s0 = t0) (H1 : s1 = t1) (H2 : s2 = t2) :
+  cLift s0 s1 s2 = cLift t0 t1 t2.
+Proof.
+exact (eq_trans
+         (eq_trans (eq_trans eq_refl (ap (fun x => cLift x s1 s2) H0))
+            (ap (fun x => cLift t0 x s2) H1))
+         (ap (fun x => cLift t0 t1 x) H2)).
+Qed.
+
+Lemma upRen_term_term (xi : nat -> nat) : nat -> nat.
+Proof.
+exact (up_ren xi).
+Defined.
+
+Fixpoint ren_ty (xi_term : nat -> nat) (s : ty) {struct s} : ty :=
+  match s with
+  | Prod s0 s1 =>
+      Prod (ren_ty xi_term s0) (ren_ty (upRen_term_term xi_term) s1)
+  | Decode s0 s1 => Decode s0 (ren_term xi_term s1)
+  | U s0 => U s0
+  end
+with ren_term (xi_term : nat -> nat) (s : term) {struct s} : term :=
+  match s with
+  | var_term s0 => var_term (xi_term s0)
+  | Lambda s0 s1 s2 =>
+      Lambda (ren_ty xi_term s0) (ren_ty (upRen_term_term xi_term) s1)
+        (ren_term (upRen_term_term xi_term) s2)
+  | App s0 s1 s2 s3 =>
+      App (ren_ty xi_term s0) (ren_ty (upRen_term_term xi_term) s1)
+        (ren_term xi_term s2) (ren_term xi_term s3)
+  | cProd s0 s1 s2 =>
+      cProd s0 (ren_term xi_term s1) (ren_term (upRen_term_term xi_term) s2)
+  | cU s0 s1 => cU s0 s1
+  | cLift s0 s1 s2 => cLift s0 s1 (ren_term xi_term s2)
+  end.
+
+Lemma up_term_term (sigma : nat -> term) : nat -> term.
+Proof.
+exact (scons (var_term var_zero) (funcomp (ren_term shift) sigma)).
+Defined.
+
+Fixpoint subst_ty (sigma_term : nat -> term) (s : ty) {struct s} : ty :=
+  match s with
+  | Prod s0 s1 =>
+      Prod (subst_ty sigma_term s0) (subst_ty (up_term_term sigma_term) s1)
+  | Decode s0 s1 => Decode s0 (subst_term sigma_term s1)
+  | U s0 => U s0
+  end
+with subst_term (sigma_term : nat -> term) (s : term) {struct s} : term :=
+  match s with
+  | var_term s0 => sigma_term s0
+  | Lambda s0 s1 s2 =>
+      Lambda (subst_ty sigma_term s0) (subst_ty (up_term_term sigma_term) s1)
+        (subst_term (up_term_term sigma_term) s2)
+  | App s0 s1 s2 s3 =>
+      App (subst_ty sigma_term s0) (subst_ty (up_term_term sigma_term) s1)
+        (subst_term sigma_term s2) (subst_term sigma_term s3)
+  | cProd s0 s1 s2 =>
+      cProd s0 (subst_term sigma_term s1)
+        (subst_term (up_term_term sigma_term) s2)
+  | cU s0 s1 => cU s0 s1
+  | cLift s0 s1 s2 => cLift s0 s1 (subst_term sigma_term s2)
+  end.
+
+Lemma upId_term_term (sigma : nat -> term)
+  (Eq : forall x, sigma x = var_term x) :
+  forall x, up_term_term sigma x = var_term x.
+Proof.
+exact (fun n =>
+       match n with
+       | S n' => ap (ren_term shift) (Eq n')
+       | O => eq_refl
+       end).
+Qed.
+
+Fixpoint idSubst_ty (sigma_term : nat -> term)
+(Eq_term : forall x, sigma_term x = var_term x) (s : ty) {struct s} :
+subst_ty sigma_term s = s :=
+  match s with
+  | Prod s0 s1 =>
+      congr_Prod (idSubst_ty sigma_term Eq_term s0)
+        (idSubst_ty (up_term_term sigma_term) (upId_term_term _ Eq_term) s1)
+  | Decode s0 s1 =>
+      congr_Decode (eq_refl s0) (idSubst_term sigma_term Eq_term s1)
+  | U s0 => congr_U (eq_refl s0)
+  end
+with idSubst_term (sigma_term : nat -> term)
+(Eq_term : forall x, sigma_term x = var_term x) (s : term) {struct s} :
+subst_term sigma_term s = s :=
+  match s with
+  | var_term s0 => Eq_term s0
+  | Lambda s0 s1 s2 =>
+      congr_Lambda (idSubst_ty sigma_term Eq_term s0)
+        (idSubst_ty (up_term_term sigma_term) (upId_term_term _ Eq_term) s1)
+        (idSubst_term (up_term_term sigma_term) (upId_term_term _ Eq_term) s2)
+  | App s0 s1 s2 s3 =>
+      congr_App (idSubst_ty sigma_term Eq_term s0)
+        (idSubst_ty (up_term_term sigma_term) (upId_term_term _ Eq_term) s1)
+        (idSubst_term sigma_term Eq_term s2)
+        (idSubst_term sigma_term Eq_term s3)
+  | cProd s0 s1 s2 =>
+      congr_cProd (eq_refl s0) (idSubst_term sigma_term Eq_term s1)
+        (idSubst_term (up_term_term sigma_term) (upId_term_term _ Eq_term) s2)
+  | cU s0 s1 => congr_cU (eq_refl s0) (eq_refl s1)
+  | cLift s0 s1 s2 =>
+      congr_cLift (eq_refl s0) (eq_refl s1)
+        (idSubst_term sigma_term Eq_term s2)
+  end.
+
+Lemma upExtRen_term_term (xi : nat -> nat) (zeta : nat -> nat)
+  (Eq : forall x, xi x = zeta x) :
+  forall x, upRen_term_term xi x = upRen_term_term zeta x.
+Proof.
+exact (fun n => match n with
+                | S n' => ap shift (Eq n')
+                | O => eq_refl
+                end).
+Qed.
+
+Fixpoint extRen_ty (xi_term : nat -> nat) (zeta_term : nat -> nat)
+(Eq_term : forall x, xi_term x = zeta_term x) (s : ty) {struct s} :
+ren_ty xi_term s = ren_ty zeta_term s :=
+  match s with
+  | Prod s0 s1 =>
+      congr_Prod (extRen_ty xi_term zeta_term Eq_term s0)
+        (extRen_ty (upRen_term_term xi_term) (upRen_term_term zeta_term)
+           (upExtRen_term_term _ _ Eq_term) s1)
+  | Decode s0 s1 =>
+      congr_Decode (eq_refl s0) (extRen_term xi_term zeta_term Eq_term s1)
+  | U s0 => congr_U (eq_refl s0)
+  end
+with extRen_term (xi_term : nat -> nat) (zeta_term : nat -> nat)
+(Eq_term : forall x, xi_term x = zeta_term x) (s : term) {struct s} :
+ren_term xi_term s = ren_term zeta_term s :=
+  match s with
+  | var_term s0 => ap (var_term) (Eq_term s0)
+  | Lambda s0 s1 s2 =>
+      congr_Lambda (extRen_ty xi_term zeta_term Eq_term s0)
+        (extRen_ty (upRen_term_term xi_term) (upRen_term_term zeta_term)
+           (upExtRen_term_term _ _ Eq_term) s1)
+        (extRen_term (upRen_term_term xi_term) (upRen_term_term zeta_term)
+           (upExtRen_term_term _ _ Eq_term) s2)
+  | App s0 s1 s2 s3 =>
+      congr_App (extRen_ty xi_term zeta_term Eq_term s0)
+        (extRen_ty (upRen_term_term xi_term) (upRen_term_term zeta_term)
+           (upExtRen_term_term _ _ Eq_term) s1)
+        (extRen_term xi_term zeta_term Eq_term s2)
+        (extRen_term xi_term zeta_term Eq_term s3)
+  | cProd s0 s1 s2 =>
+      congr_cProd (eq_refl s0) (extRen_term xi_term zeta_term Eq_term s1)
+        (extRen_term (upRen_term_term xi_term) (upRen_term_term zeta_term)
+           (upExtRen_term_term _ _ Eq_term) s2)
+  | cU s0 s1 => congr_cU (eq_refl s0) (eq_refl s1)
+  | cLift s0 s1 s2 =>
+      congr_cLift (eq_refl s0) (eq_refl s1)
+        (extRen_term xi_term zeta_term Eq_term s2)
+  end.
+
+Lemma upExt_term_term (sigma : nat -> term) (tau : nat -> term)
+  (Eq : forall x, sigma x = tau x) :
+  forall x, up_term_term sigma x = up_term_term tau x.
+Proof.
+exact (fun n =>
+       match n with
+       | S n' => ap (ren_term shift) (Eq n')
+       | O => eq_refl
+       end).
+Qed.
+
+Fixpoint ext_ty (sigma_term : nat -> term) (tau_term : nat -> term)
+(Eq_term : forall x, sigma_term x = tau_term x) (s : ty) {struct s} :
+subst_ty sigma_term s = subst_ty tau_term s :=
+  match s with
+  | Prod s0 s1 =>
+      congr_Prod (ext_ty sigma_term tau_term Eq_term s0)
+        (ext_ty (up_term_term sigma_term) (up_term_term tau_term)
+           (upExt_term_term _ _ Eq_term) s1)
+  | Decode s0 s1 =>
+      congr_Decode (eq_refl s0) (ext_term sigma_term tau_term Eq_term s1)
+  | U s0 => congr_U (eq_refl s0)
+  end
+with ext_term (sigma_term : nat -> term) (tau_term : nat -> term)
+(Eq_term : forall x, sigma_term x = tau_term x) (s : term) {struct s} :
+subst_term sigma_term s = subst_term tau_term s :=
+  match s with
+  | var_term s0 => Eq_term s0
+  | Lambda s0 s1 s2 =>
+      congr_Lambda (ext_ty sigma_term tau_term Eq_term s0)
+        (ext_ty (up_term_term sigma_term) (up_term_term tau_term)
+           (upExt_term_term _ _ Eq_term) s1)
+        (ext_term (up_term_term sigma_term) (up_term_term tau_term)
+           (upExt_term_term _ _ Eq_term) s2)
+  | App s0 s1 s2 s3 =>
+      congr_App (ext_ty sigma_term tau_term Eq_term s0)
+        (ext_ty (up_term_term sigma_term) (up_term_term tau_term)
+           (upExt_term_term _ _ Eq_term) s1)
+        (ext_term sigma_term tau_term Eq_term s2)
+        (ext_term sigma_term tau_term Eq_term s3)
+  | cProd s0 s1 s2 =>
+      congr_cProd (eq_refl s0) (ext_term sigma_term tau_term Eq_term s1)
+        (ext_term (up_term_term sigma_term) (up_term_term tau_term)
+           (upExt_term_term _ _ Eq_term) s2)
+  | cU s0 s1 => congr_cU (eq_refl s0) (eq_refl s1)
+  | cLift s0 s1 s2 =>
+      congr_cLift (eq_refl s0) (eq_refl s1)
+        (ext_term sigma_term tau_term Eq_term s2)
+  end.
+
+Lemma up_ren_ren_term_term (xi : nat -> nat) (zeta : nat -> nat)
+  (rho : nat -> nat) (Eq : forall x, funcomp zeta xi x = rho x) :
+  forall x,
+  funcomp (upRen_term_term zeta) (upRen_term_term xi) x =
+  upRen_term_term rho x.
+Proof.
+exact (up_ren_ren xi zeta rho Eq).
+Qed.
+
+Fixpoint compRenRen_ty (xi_term : nat -> nat) (zeta_term : nat -> nat)
+(rho_term : nat -> nat)
+(Eq_term : forall x, funcomp zeta_term xi_term x = rho_term x) (s : ty)
+{struct s} : ren_ty zeta_term (ren_ty xi_term s) = ren_ty rho_term s :=
+  match s with
+  | Prod s0 s1 =>
+      congr_Prod (compRenRen_ty xi_term zeta_term rho_term Eq_term s0)
+        (compRenRen_ty (upRen_term_term xi_term) (upRen_term_term zeta_term)
+           (upRen_term_term rho_term) (up_ren_ren _ _ _ Eq_term) s1)
+  | Decode s0 s1 =>
+      congr_Decode (eq_refl s0)
+        (compRenRen_term xi_term zeta_term rho_term Eq_term s1)
+  | U s0 => congr_U (eq_refl s0)
+  end
+with compRenRen_term (xi_term : nat -> nat) (zeta_term : nat -> nat)
+(rho_term : nat -> nat)
+(Eq_term : forall x, funcomp zeta_term xi_term x = rho_term x) (s : term)
+{struct s} : ren_term zeta_term (ren_term xi_term s) = ren_term rho_term s :=
+  match s with
+  | var_term s0 => ap (var_term) (Eq_term s0)
+  | Lambda s0 s1 s2 =>
+      congr_Lambda (compRenRen_ty xi_term zeta_term rho_term Eq_term s0)
+        (compRenRen_ty (upRen_term_term xi_term) (upRen_term_term zeta_term)
+           (upRen_term_term rho_term) (up_ren_ren _ _ _ Eq_term) s1)
+        (compRenRen_term (upRen_term_term xi_term)
+           (upRen_term_term zeta_term) (upRen_term_term rho_term)
+           (up_ren_ren _ _ _ Eq_term) s2)
+  | App s0 s1 s2 s3 =>
+      congr_App (compRenRen_ty xi_term zeta_term rho_term Eq_term s0)
+        (compRenRen_ty (upRen_term_term xi_term) (upRen_term_term zeta_term)
+           (upRen_term_term rho_term) (up_ren_ren _ _ _ Eq_term) s1)
+        (compRenRen_term xi_term zeta_term rho_term Eq_term s2)
+        (compRenRen_term xi_term zeta_term rho_term Eq_term s3)
+  | cProd s0 s1 s2 =>
+      congr_cProd (eq_refl s0)
+        (compRenRen_term xi_term zeta_term rho_term Eq_term s1)
+        (compRenRen_term (upRen_term_term xi_term)
+           (upRen_term_term zeta_term) (upRen_term_term rho_term)
+           (up_ren_ren _ _ _ Eq_term) s2)
+  | cU s0 s1 => congr_cU (eq_refl s0) (eq_refl s1)
+  | cLift s0 s1 s2 =>
+      congr_cLift (eq_refl s0) (eq_refl s1)
+        (compRenRen_term xi_term zeta_term rho_term Eq_term s2)
+  end.
+
+Lemma up_ren_subst_term_term (xi : nat -> nat) (tau : nat -> term)
+  (theta : nat -> term) (Eq : forall x, funcomp tau xi x = theta x) :
+  forall x,
+  funcomp (up_term_term tau) (upRen_term_term xi) x = up_term_term theta x.
+Proof.
+exact (fun n =>
+       match n with
+       | S n' => ap (ren_term shift) (Eq n')
+       | O => eq_refl
+       end).
+Qed.
+
+Fixpoint compRenSubst_ty (xi_term : nat -> nat) (tau_term : nat -> term)
+(theta_term : nat -> term)
+(Eq_term : forall x, funcomp tau_term xi_term x = theta_term x) (s : ty)
+{struct s} : subst_ty tau_term (ren_ty xi_term s) = subst_ty theta_term s :=
+  match s with
+  | Prod s0 s1 =>
+      congr_Prod (compRenSubst_ty xi_term tau_term theta_term Eq_term s0)
+        (compRenSubst_ty (upRen_term_term xi_term) (up_term_term tau_term)
+           (up_term_term theta_term) (up_ren_subst_term_term _ _ _ Eq_term)
+           s1)
+  | Decode s0 s1 =>
+      congr_Decode (eq_refl s0)
+        (compRenSubst_term xi_term tau_term theta_term Eq_term s1)
+  | U s0 => congr_U (eq_refl s0)
+  end
+with compRenSubst_term (xi_term : nat -> nat) (tau_term : nat -> term)
+(theta_term : nat -> term)
+(Eq_term : forall x, funcomp tau_term xi_term x = theta_term x) (s : term)
+{struct s} :
+subst_term tau_term (ren_term xi_term s) = subst_term theta_term s :=
+  match s with
+  | var_term s0 => Eq_term s0
+  | Lambda s0 s1 s2 =>
+      congr_Lambda (compRenSubst_ty xi_term tau_term theta_term Eq_term s0)
+        (compRenSubst_ty (upRen_term_term xi_term) (up_term_term tau_term)
+           (up_term_term theta_term) (up_ren_subst_term_term _ _ _ Eq_term)
+           s1)
+        (compRenSubst_term (upRen_term_term xi_term) (up_term_term tau_term)
+           (up_term_term theta_term) (up_ren_subst_term_term _ _ _ Eq_term)
+           s2)
+  | App s0 s1 s2 s3 =>
+      congr_App (compRenSubst_ty xi_term tau_term theta_term Eq_term s0)
+        (compRenSubst_ty (upRen_term_term xi_term) (up_term_term tau_term)
+           (up_term_term theta_term) (up_ren_subst_term_term _ _ _ Eq_term)
+           s1) (compRenSubst_term xi_term tau_term theta_term Eq_term s2)
+        (compRenSubst_term xi_term tau_term theta_term Eq_term s3)
+  | cProd s0 s1 s2 =>
+      congr_cProd (eq_refl s0)
+        (compRenSubst_term xi_term tau_term theta_term Eq_term s1)
+        (compRenSubst_term (upRen_term_term xi_term) (up_term_term tau_term)
+           (up_term_term theta_term) (up_ren_subst_term_term _ _ _ Eq_term)
+           s2)
+  | cU s0 s1 => congr_cU (eq_refl s0) (eq_refl s1)
+  | cLift s0 s1 s2 =>
+      congr_cLift (eq_refl s0) (eq_refl s1)
+        (compRenSubst_term xi_term tau_term theta_term Eq_term s2)
+  end.
+
+Lemma up_subst_ren_term_term (sigma : nat -> term) (zeta_term : nat -> nat)
+  (theta : nat -> term)
+  (Eq : forall x, funcomp (ren_term zeta_term) sigma x = theta x) :
+  forall x,
+  funcomp (ren_term (upRen_term_term zeta_term)) (up_term_term sigma) x =
+  up_term_term theta x.
+Proof.
+exact (fun n =>
+       match n with
+       | S n' =>
+           eq_trans
+             (compRenRen_term shift (upRen_term_term zeta_term)
+                (funcomp shift zeta_term) (fun x => eq_refl) (sigma n'))
+             (eq_trans
+                (eq_sym
+                   (compRenRen_term zeta_term shift (funcomp shift zeta_term)
+                      (fun x => eq_refl) (sigma n')))
+                (ap (ren_term shift) (Eq n')))
+       | O => eq_refl
+       end).
+Qed.
+
+Fixpoint compSubstRen_ty (sigma_term : nat -> term) (zeta_term : nat -> nat)
+(theta_term : nat -> term)
+(Eq_term : forall x, funcomp (ren_term zeta_term) sigma_term x = theta_term x)
+(s : ty) {struct s} :
+ren_ty zeta_term (subst_ty sigma_term s) = subst_ty theta_term s :=
+  match s with
+  | Prod s0 s1 =>
+      congr_Prod (compSubstRen_ty sigma_term zeta_term theta_term Eq_term s0)
+        (compSubstRen_ty (up_term_term sigma_term)
+           (upRen_term_term zeta_term) (up_term_term theta_term)
+           (up_subst_ren_term_term _ _ _ Eq_term) s1)
+  | Decode s0 s1 =>
+      congr_Decode (eq_refl s0)
+        (compSubstRen_term sigma_term zeta_term theta_term Eq_term s1)
+  | U s0 => congr_U (eq_refl s0)
+  end
+with compSubstRen_term (sigma_term : nat -> term) (zeta_term : nat -> nat)
+(theta_term : nat -> term)
+(Eq_term : forall x, funcomp (ren_term zeta_term) sigma_term x = theta_term x)
+(s : term) {struct s} :
+ren_term zeta_term (subst_term sigma_term s) = subst_term theta_term s :=
+  match s with
+  | var_term s0 => Eq_term s0
+  | Lambda s0 s1 s2 =>
+      congr_Lambda
+        (compSubstRen_ty sigma_term zeta_term theta_term Eq_term s0)
+        (compSubstRen_ty (up_term_term sigma_term)
+           (upRen_term_term zeta_term) (up_term_term theta_term)
+           (up_subst_ren_term_term _ _ _ Eq_term) s1)
+        (compSubstRen_term (up_term_term sigma_term)
+           (upRen_term_term zeta_term) (up_term_term theta_term)
+           (up_subst_ren_term_term _ _ _ Eq_term) s2)
+  | App s0 s1 s2 s3 =>
+      congr_App (compSubstRen_ty sigma_term zeta_term theta_term Eq_term s0)
+        (compSubstRen_ty (up_term_term sigma_term)
+           (upRen_term_term zeta_term) (up_term_term theta_term)
+           (up_subst_ren_term_term _ _ _ Eq_term) s1)
+        (compSubstRen_term sigma_term zeta_term theta_term Eq_term s2)
+        (compSubstRen_term sigma_term zeta_term theta_term Eq_term s3)
+  | cProd s0 s1 s2 =>
+      congr_cProd (eq_refl s0)
+        (compSubstRen_term sigma_term zeta_term theta_term Eq_term s1)
+        (compSubstRen_term (up_term_term sigma_term)
+           (upRen_term_term zeta_term) (up_term_term theta_term)
+           (up_subst_ren_term_term _ _ _ Eq_term) s2)
+  | cU s0 s1 => congr_cU (eq_refl s0) (eq_refl s1)
+  | cLift s0 s1 s2 =>
+      congr_cLift (eq_refl s0) (eq_refl s1)
+        (compSubstRen_term sigma_term zeta_term theta_term Eq_term s2)
+  end.
+
+Lemma up_subst_subst_term_term (sigma : nat -> term) (tau_term : nat -> term)
+  (theta : nat -> term)
+  (Eq : forall x, funcomp (subst_term tau_term) sigma x = theta x) :
+  forall x,
+  funcomp (subst_term (up_term_term tau_term)) (up_term_term sigma) x =
+  up_term_term theta x.
+Proof.
+exact (fun n =>
+       match n with
+       | S n' =>
+           eq_trans
+             (compRenSubst_term shift (up_term_term tau_term)
+                (funcomp (up_term_term tau_term) shift) (fun x => eq_refl)
+                (sigma n'))
+             (eq_trans
+                (eq_sym
+                   (compSubstRen_term tau_term shift
+                      (funcomp (ren_term shift) tau_term) (fun x => eq_refl)
+                      (sigma n'))) (ap (ren_term shift) (Eq n')))
+       | O => eq_refl
+       end).
+Qed.
+
+Fixpoint compSubstSubst_ty (sigma_term : nat -> term)
+(tau_term : nat -> term) (theta_term : nat -> term)
+(Eq_term : forall x,
+           funcomp (subst_term tau_term) sigma_term x = theta_term x)
+(s : ty) {struct s} :
+subst_ty tau_term (subst_ty sigma_term s) = subst_ty theta_term s :=
+  match s with
+  | Prod s0 s1 =>
+      congr_Prod
+        (compSubstSubst_ty sigma_term tau_term theta_term Eq_term s0)
+        (compSubstSubst_ty (up_term_term sigma_term) (up_term_term tau_term)
+           (up_term_term theta_term) (up_subst_subst_term_term _ _ _ Eq_term)
+           s1)
+  | Decode s0 s1 =>
+      congr_Decode (eq_refl s0)
+        (compSubstSubst_term sigma_term tau_term theta_term Eq_term s1)
+  | U s0 => congr_U (eq_refl s0)
+  end
+with compSubstSubst_term (sigma_term : nat -> term) (tau_term : nat -> term)
+(theta_term : nat -> term)
+(Eq_term : forall x,
+           funcomp (subst_term tau_term) sigma_term x = theta_term x)
+(s : term) {struct s} :
+subst_term tau_term (subst_term sigma_term s) = subst_term theta_term s :=
+  match s with
+  | var_term s0 => Eq_term s0
+  | Lambda s0 s1 s2 =>
+      congr_Lambda
+        (compSubstSubst_ty sigma_term tau_term theta_term Eq_term s0)
+        (compSubstSubst_ty (up_term_term sigma_term) (up_term_term tau_term)
+           (up_term_term theta_term) (up_subst_subst_term_term _ _ _ Eq_term)
+           s1)
+        (compSubstSubst_term (up_term_term sigma_term)
+           (up_term_term tau_term) (up_term_term theta_term)
+           (up_subst_subst_term_term _ _ _ Eq_term) s2)
+  | App s0 s1 s2 s3 =>
+      congr_App (compSubstSubst_ty sigma_term tau_term theta_term Eq_term s0)
+        (compSubstSubst_ty (up_term_term sigma_term) (up_term_term tau_term)
+           (up_term_term theta_term) (up_subst_subst_term_term _ _ _ Eq_term)
+           s1)
+        (compSubstSubst_term sigma_term tau_term theta_term Eq_term s2)
+        (compSubstSubst_term sigma_term tau_term theta_term Eq_term s3)
+  | cProd s0 s1 s2 =>
+      congr_cProd (eq_refl s0)
+        (compSubstSubst_term sigma_term tau_term theta_term Eq_term s1)
+        (compSubstSubst_term (up_term_term sigma_term)
+           (up_term_term tau_term) (up_term_term theta_term)
+           (up_subst_subst_term_term _ _ _ Eq_term) s2)
+  | cU s0 s1 => congr_cU (eq_refl s0) (eq_refl s1)
+  | cLift s0 s1 s2 =>
+      congr_cLift (eq_refl s0) (eq_refl s1)
+        (compSubstSubst_term sigma_term tau_term theta_term Eq_term s2)
+  end.
+
+Lemma renRen_ty (xi_term : nat -> nat) (zeta_term : nat -> nat) (s : ty) :
+  ren_ty zeta_term (ren_ty xi_term s) = ren_ty (funcomp zeta_term xi_term) s.
+Proof.
+exact (compRenRen_ty xi_term zeta_term _ (fun n => eq_refl) s).
+Qed.
+
+Lemma renRen'_ty_pointwise (xi_term : nat -> nat) (zeta_term : nat -> nat) :
+  pointwise_relation _ eq (funcomp (ren_ty zeta_term) (ren_ty xi_term))
+    (ren_ty (funcomp zeta_term xi_term)).
+Proof.
+exact (fun s => compRenRen_ty xi_term zeta_term _ (fun n => eq_refl) s).
+Qed.
+
+Lemma renRen_term (xi_term : nat -> nat) (zeta_term : nat -> nat) (s : term)
+  :
+  ren_term zeta_term (ren_term xi_term s) =
+  ren_term (funcomp zeta_term xi_term) s.
+Proof.
+exact (compRenRen_term xi_term zeta_term _ (fun n => eq_refl) s).
+Qed.
+
+Lemma renRen'_term_pointwise (xi_term : nat -> nat) (zeta_term : nat -> nat)
+  :
+  pointwise_relation _ eq (funcomp (ren_term zeta_term) (ren_term xi_term))
+    (ren_term (funcomp zeta_term xi_term)).
+Proof.
+exact (fun s => compRenRen_term xi_term zeta_term _ (fun n => eq_refl) s).
+Qed.
+
+Lemma renSubst_ty (xi_term : nat -> nat) (tau_term : nat -> term) (s : ty) :
+  subst_ty tau_term (ren_ty xi_term s) =
+  subst_ty (funcomp tau_term xi_term) s.
+Proof.
+exact (compRenSubst_ty xi_term tau_term _ (fun n => eq_refl) s).
+Qed.
+
+Lemma renSubst_ty_pointwise (xi_term : nat -> nat) (tau_term : nat -> term) :
+  pointwise_relation _ eq (funcomp (subst_ty tau_term) (ren_ty xi_term))
+    (subst_ty (funcomp tau_term xi_term)).
+Proof.
+exact (fun s => compRenSubst_ty xi_term tau_term _ (fun n => eq_refl) s).
+Qed.
+
+Lemma renSubst_term (xi_term : nat -> nat) (tau_term : nat -> term)
+  (s : term) :
+  subst_term tau_term (ren_term xi_term s) =
+  subst_term (funcomp tau_term xi_term) s.
+Proof.
+exact (compRenSubst_term xi_term tau_term _ (fun n => eq_refl) s).
+Qed.
+
+Lemma renSubst_term_pointwise (xi_term : nat -> nat) (tau_term : nat -> term)
+  :
+  pointwise_relation _ eq (funcomp (subst_term tau_term) (ren_term xi_term))
+    (subst_term (funcomp tau_term xi_term)).
+Proof.
+exact (fun s => compRenSubst_term xi_term tau_term _ (fun n => eq_refl) s).
+Qed.
+
+Lemma substRen_ty (sigma_term : nat -> term) (zeta_term : nat -> nat)
+  (s : ty) :
+  ren_ty zeta_term (subst_ty sigma_term s) =
+  subst_ty (funcomp (ren_term zeta_term) sigma_term) s.
+Proof.
+exact (compSubstRen_ty sigma_term zeta_term _ (fun n => eq_refl) s).
+Qed.
+
+Lemma substRen_ty_pointwise (sigma_term : nat -> term)
+  (zeta_term : nat -> nat) :
+  pointwise_relation _ eq (funcomp (ren_ty zeta_term) (subst_ty sigma_term))
+    (subst_ty (funcomp (ren_term zeta_term) sigma_term)).
+Proof.
+exact (fun s => compSubstRen_ty sigma_term zeta_term _ (fun n => eq_refl) s).
+Qed.
+
+Lemma substRen_term (sigma_term : nat -> term) (zeta_term : nat -> nat)
+  (s : term) :
+  ren_term zeta_term (subst_term sigma_term s) =
+  subst_term (funcomp (ren_term zeta_term) sigma_term) s.
+Proof.
+exact (compSubstRen_term sigma_term zeta_term _ (fun n => eq_refl) s).
+Qed.
+
+Lemma substRen_term_pointwise (sigma_term : nat -> term)
+  (zeta_term : nat -> nat) :
+  pointwise_relation _ eq
+    (funcomp (ren_term zeta_term) (subst_term sigma_term))
+    (subst_term (funcomp (ren_term zeta_term) sigma_term)).
+Proof.
+exact (fun s => compSubstRen_term sigma_term zeta_term _ (fun n => eq_refl) s).
+Qed.
+
+Lemma substSubst_ty (sigma_term : nat -> term) (tau_term : nat -> term)
+  (s : ty) :
+  subst_ty tau_term (subst_ty sigma_term s) =
+  subst_ty (funcomp (subst_term tau_term) sigma_term) s.
+Proof.
+exact (compSubstSubst_ty sigma_term tau_term _ (fun n => eq_refl) s).
+Qed.
+
+Lemma substSubst_ty_pointwise (sigma_term : nat -> term)
+  (tau_term : nat -> term) :
+  pointwise_relation _ eq (funcomp (subst_ty tau_term) (subst_ty sigma_term))
+    (subst_ty (funcomp (subst_term tau_term) sigma_term)).
+Proof.
+exact (fun s => compSubstSubst_ty sigma_term tau_term _ (fun n => eq_refl) s).
+Qed.
+
+Lemma substSubst_term (sigma_term : nat -> term) (tau_term : nat -> term)
+  (s : term) :
+  subst_term tau_term (subst_term sigma_term s) =
+  subst_term (funcomp (subst_term tau_term) sigma_term) s.
+Proof.
+exact (compSubstSubst_term sigma_term tau_term _ (fun n => eq_refl) s).
+Qed.
+
+Lemma substSubst_term_pointwise (sigma_term : nat -> term)
+  (tau_term : nat -> term) :
+  pointwise_relation _ eq
+    (funcomp (subst_term tau_term) (subst_term sigma_term))
+    (subst_term (funcomp (subst_term tau_term) sigma_term)).
+Proof.
+exact (fun s =>
+       compSubstSubst_term sigma_term tau_term _ (fun n => eq_refl) s).
+Qed.
+
+Lemma rinstInst_up_term_term (xi : nat -> nat) (sigma : nat -> term)
+  (Eq : forall x, funcomp (var_term) xi x = sigma x) :
+  forall x, funcomp (var_term) (upRen_term_term xi) x = up_term_term sigma x.
+Proof.
+exact (fun n =>
+       match n with
+       | S n' => ap (ren_term shift) (Eq n')
+       | O => eq_refl
+       end).
+Qed.
+
+Fixpoint rinst_inst_ty (xi_term : nat -> nat) (sigma_term : nat -> term)
+(Eq_term : forall x, funcomp (var_term) xi_term x = sigma_term x) (s : ty)
+{struct s} : ren_ty xi_term s = subst_ty sigma_term s :=
+  match s with
+  | Prod s0 s1 =>
+      congr_Prod (rinst_inst_ty xi_term sigma_term Eq_term s0)
+        (rinst_inst_ty (upRen_term_term xi_term) (up_term_term sigma_term)
+           (rinstInst_up_term_term _ _ Eq_term) s1)
+  | Decode s0 s1 =>
+      congr_Decode (eq_refl s0)
+        (rinst_inst_term xi_term sigma_term Eq_term s1)
+  | U s0 => congr_U (eq_refl s0)
+  end
+with rinst_inst_term (xi_term : nat -> nat) (sigma_term : nat -> term)
+(Eq_term : forall x, funcomp (var_term) xi_term x = sigma_term x) (s : term)
+{struct s} : ren_term xi_term s = subst_term sigma_term s :=
+  match s with
+  | var_term s0 => Eq_term s0
+  | Lambda s0 s1 s2 =>
+      congr_Lambda (rinst_inst_ty xi_term sigma_term Eq_term s0)
+        (rinst_inst_ty (upRen_term_term xi_term) (up_term_term sigma_term)
+           (rinstInst_up_term_term _ _ Eq_term) s1)
+        (rinst_inst_term (upRen_term_term xi_term) (up_term_term sigma_term)
+           (rinstInst_up_term_term _ _ Eq_term) s2)
+  | App s0 s1 s2 s3 =>
+      congr_App (rinst_inst_ty xi_term sigma_term Eq_term s0)
+        (rinst_inst_ty (upRen_term_term xi_term) (up_term_term sigma_term)
+           (rinstInst_up_term_term _ _ Eq_term) s1)
+        (rinst_inst_term xi_term sigma_term Eq_term s2)
+        (rinst_inst_term xi_term sigma_term Eq_term s3)
+  | cProd s0 s1 s2 =>
+      congr_cProd (eq_refl s0)
+        (rinst_inst_term xi_term sigma_term Eq_term s1)
+        (rinst_inst_term (upRen_term_term xi_term) (up_term_term sigma_term)
+           (rinstInst_up_term_term _ _ Eq_term) s2)
+  | cU s0 s1 => congr_cU (eq_refl s0) (eq_refl s1)
+  | cLift s0 s1 s2 =>
+      congr_cLift (eq_refl s0) (eq_refl s1)
+        (rinst_inst_term xi_term sigma_term Eq_term s2)
+  end.
+
+Lemma rinstInst'_ty (xi_term : nat -> nat) (s : ty) :
+  ren_ty xi_term s = subst_ty (funcomp (var_term) xi_term) s.
+Proof.
+exact (rinst_inst_ty xi_term _ (fun n => eq_refl) s).
+Qed.
+
+Lemma rinstInst'_ty_pointwise (xi_term : nat -> nat) :
+  pointwise_relation _ eq (ren_ty xi_term)
+    (subst_ty (funcomp (var_term) xi_term)).
+Proof.
+exact (fun s => rinst_inst_ty xi_term _ (fun n => eq_refl) s).
+Qed.
+
+Lemma rinstInst'_term (xi_term : nat -> nat) (s : term) :
+  ren_term xi_term s = subst_term (funcomp (var_term) xi_term) s.
+Proof.
+exact (rinst_inst_term xi_term _ (fun n => eq_refl) s).
+Qed.
+
+Lemma rinstInst'_term_pointwise (xi_term : nat -> nat) :
+  pointwise_relation _ eq (ren_term xi_term)
+    (subst_term (funcomp (var_term) xi_term)).
+Proof.
+exact (fun s => rinst_inst_term xi_term _ (fun n => eq_refl) s).
+Qed.
+
+Lemma instId'_ty (s : ty) : subst_ty (var_term) s = s.
+Proof.
+exact (idSubst_ty (var_term) (fun n => eq_refl) s).
+Qed.
+
+Lemma instId'_ty_pointwise : pointwise_relation _ eq (subst_ty (var_term)) id.
+Proof.
+exact (fun s => idSubst_ty (var_term) (fun n => eq_refl) s).
+Qed.
+
+Lemma instId'_term (s : term) : subst_term (var_term) s = s.
+Proof.
+exact (idSubst_term (var_term) (fun n => eq_refl) s).
+Qed.
+
+Lemma instId'_term_pointwise :
+  pointwise_relation _ eq (subst_term (var_term)) id.
+Proof.
+exact (fun s => idSubst_term (var_term) (fun n => eq_refl) s).
+Qed.
+
+Lemma rinstId'_ty (s : ty) : ren_ty id s = s.
+Proof.
+exact (eq_ind_r (fun t => t = s) (instId'_ty s) (rinstInst'_ty id s)).
+Qed.
+
+Lemma rinstId'_ty_pointwise : pointwise_relation _ eq (@ren_ty id) id.
+Proof.
+exact (fun s => eq_ind_r (fun t => t = s) (instId'_ty s) (rinstInst'_ty id s)).
+Qed.
+
+Lemma rinstId'_term (s : term) : ren_term id s = s.
+Proof.
+exact (eq_ind_r (fun t => t = s) (instId'_term s) (rinstInst'_term id s)).
+Qed.
+
+Lemma rinstId'_term_pointwise : pointwise_relation _ eq (@ren_term id) id.
+Proof.
+exact (fun s =>
+       eq_ind_r (fun t => t = s) (instId'_term s) (rinstInst'_term id s)).
+Qed.
+
+Lemma varL'_term (sigma_term : nat -> term) (x : nat) :
+  subst_term sigma_term (var_term x) = sigma_term x.
+Proof.
+exact (eq_refl).
+Qed.
+
+Lemma varL'_term_pointwise (sigma_term : nat -> term) :
+  pointwise_relation _ eq (funcomp (subst_term sigma_term) (var_term))
+    sigma_term.
+Proof.
+exact (fun x => eq_refl).
+Qed.
+
+Lemma varLRen'_term (xi_term : nat -> nat) (x : nat) :
+  ren_term xi_term (var_term x) = var_term (xi_term x).
+Proof.
+exact (eq_refl).
+Qed.
+
+Lemma varLRen'_term_pointwise (xi_term : nat -> nat) :
+  pointwise_relation _ eq (funcomp (ren_term xi_term) (var_term))
+    (funcomp (var_term) xi_term).
+Proof.
+exact (fun x => eq_refl).
+Qed.
+
+Class Up_term X Y :=
+    up_term : X -> Y.
+
+Class Up_ty X Y :=
+    up_ty : X -> Y.
+
+Class Up_russ_term X Y :=
+    up_russ_term : X -> Y.
+
+#[global] Instance Subst_term : (Subst1 _ _ _) := @subst_term.
+
+#[global] Instance Subst_ty : (Subst1 _ _ _) := @subst_ty.
+
+#[global] Instance Up_term_term : (Up_term _ _) := @up_term_term.
+
+#[global] Instance Ren_term : (Ren1 _ _ _) := @ren_term.
+
+#[global] Instance Ren_ty : (Ren1 _ _ _) := @ren_ty.
+
+#[global] Instance VarInstance_term : (Var _ _) := @var_term.
+
+#[global]
+Instance Subst_russ_term : (Subst1 _ _ _) := @subst_russ_term.
+
+#[global]
+Instance Up_russ_term_russ_term : (Up_russ_term _ _) :=
+ @up_russ_term_russ_term.
+
+#[global] Instance Ren_russ_term : (Ren1 _ _ _) := @ren_russ_term.
+
+#[global]
+Instance VarInstance_russ_term : (Var _ _) := @r_var_term.
+
+Notation "s [ sigma_term ]" := (subst_term sigma_term s)
+( at level 7, left associativity, only printing)  : subst_scope.
+
+Notation "↑__term" := up_term (only printing)  : subst_scope.
+
+Notation "s [ sigma_term ]" := (subst_ty sigma_term s)
+( at level 7, left associativity, only printing)  : subst_scope.
+
+Notation "↑__ty" := up_ty (only printing)  : subst_scope.
+
+Notation "↑__term" := up_term_term (only printing)  : subst_scope.
+
+Notation "s ⟨ xi_term ⟩" := (ren_term xi_term s)
+( at level 7, left associativity, only printing)  : subst_scope.
+
+Notation "s ⟨ xi_term ⟩" := (ren_ty xi_term s)
+( at level 7, left associativity, only printing)  : subst_scope.
+
+Notation "'var'" := var_term ( at level 1, only printing)  : subst_scope.
+
+Notation "x '__term'" := (@ids _ _ VarInstance_term x)
+( at level 5, format "x __term", only printing)  : subst_scope.
+
+Notation "x '__term'" := (var_term x) ( at level 5, format "x __term")  :
+subst_scope.
+
+Notation "s [ sigma_russ_term ]" := (subst_russ_term sigma_russ_term s)
+( at level 7, left associativity, only printing)  : subst_scope.
+
+Notation "↑__russ_term" := up_russ_term (only printing)  : subst_scope.
+
+Notation "↑__russ_term" := up_russ_term_russ_term (only printing)  :
+subst_scope.
+
+Notation "s ⟨ xi_russ_term ⟩" := (ren_russ_term xi_russ_term s)
+( at level 7, left associativity, only printing)  : subst_scope.
+
+Notation "'var'" := r_var_term ( at level 1, only printing)  : subst_scope.
+
+Notation "x '__russ_term'" := (@ids _ _ VarInstance_russ_term x)
+( at level 5, format "x __russ_term", only printing)  : subst_scope.
+
+Notation "x '__russ_term'" := (r_var_term x)
+( at level 5, format "x __russ_term")  : subst_scope.
+
+#[global]
+Instance subst_term_morphism :
+ (Proper (respectful (pointwise_relation _ eq) (respectful eq eq))
+    (@subst_term)).
+Proof.
+exact (fun f_term g_term Eq_term s t Eq_st =>
+       eq_ind s (fun t' => subst_term f_term s = subst_term g_term t')
+         (ext_term f_term g_term Eq_term s) t Eq_st).
+Qed.
+
+#[global]
+Instance subst_term_morphism2 :
+ (Proper (respectful (pointwise_relation _ eq) (pointwise_relation _ eq))
+    (@subst_term)).
+Proof.
+exact (fun f_term g_term Eq_term s => ext_term f_term g_term Eq_term s).
+Qed.
+
+#[global]
+Instance subst_ty_morphism :
+ (Proper (respectful (pointwise_relation _ eq) (respectful eq eq))
+    (@subst_ty)).
+Proof.
+exact (fun f_term g_term Eq_term s t Eq_st =>
+       eq_ind s (fun t' => subst_ty f_term s = subst_ty g_term t')
+         (ext_ty f_term g_term Eq_term s) t Eq_st).
+Qed.
+
+#[global]
+Instance subst_ty_morphism2 :
+ (Proper (respectful (pointwise_relation _ eq) (pointwise_relation _ eq))
+    (@subst_ty)).
+Proof.
+exact (fun f_term g_term Eq_term s => ext_ty f_term g_term Eq_term s).
+Qed.
+
+#[global]
+Instance ren_term_morphism :
+ (Proper (respectful (pointwise_relation _ eq) (respectful eq eq))
+    (@ren_term)).
+Proof.
+exact (fun f_term g_term Eq_term s t Eq_st =>
+       eq_ind s (fun t' => ren_term f_term s = ren_term g_term t')
+         (extRen_term f_term g_term Eq_term s) t Eq_st).
+Qed.
+
+#[global]
+Instance ren_term_morphism2 :
+ (Proper (respectful (pointwise_relation _ eq) (pointwise_relation _ eq))
+    (@ren_term)).
+Proof.
+exact (fun f_term g_term Eq_term s => extRen_term f_term g_term Eq_term s).
+Qed.
+
+#[global]
+Instance ren_ty_morphism :
+ (Proper (respectful (pointwise_relation _ eq) (respectful eq eq)) (@ren_ty)).
+Proof.
+exact (fun f_term g_term Eq_term s t Eq_st =>
+       eq_ind s (fun t' => ren_ty f_term s = ren_ty g_term t')
+         (extRen_ty f_term g_term Eq_term s) t Eq_st).
+Qed.
+
+#[global]
+Instance ren_ty_morphism2 :
+ (Proper (respectful (pointwise_relation _ eq) (pointwise_relation _ eq))
+    (@ren_ty)).
+Proof.
+exact (fun f_term g_term Eq_term s => extRen_ty f_term g_term Eq_term s).
+Qed.
+
+#[global]
+Instance subst_russ_term_morphism :
+ (Proper (respectful (pointwise_relation _ eq) (respectful eq eq))
+    (@subst_russ_term)).
+Proof.
+exact (fun f_russ_term g_russ_term Eq_russ_term s t Eq_st =>
+       eq_ind s
+         (fun t' =>
+          subst_russ_term f_russ_term s = subst_russ_term g_russ_term t')
+         (ext_russ_term f_russ_term g_russ_term Eq_russ_term s) t Eq_st).
+Qed.
+
+#[global]
+Instance subst_russ_term_morphism2 :
+ (Proper (respectful (pointwise_relation _ eq) (pointwise_relation _ eq))
+    (@subst_russ_term)).
+Proof.
+exact (fun f_russ_term g_russ_term Eq_russ_term s =>
+       ext_russ_term f_russ_term g_russ_term Eq_russ_term s).
+Qed.
+
+#[global]
+Instance ren_russ_term_morphism :
+ (Proper (respectful (pointwise_relation _ eq) (respectful eq eq))
+    (@ren_russ_term)).
+Proof.
+exact (fun f_russ_term g_russ_term Eq_russ_term s t Eq_st =>
+       eq_ind s
+         (fun t' =>
+          ren_russ_term f_russ_term s = ren_russ_term g_russ_term t')
+         (extRen_russ_term f_russ_term g_russ_term Eq_russ_term s) t Eq_st).
+Qed.
+
+#[global]
+Instance ren_russ_term_morphism2 :
+ (Proper (respectful (pointwise_relation _ eq) (pointwise_relation _ eq))
+    (@ren_russ_term)).
+Proof.
+exact (fun f_russ_term g_russ_term Eq_russ_term s =>
+       extRen_russ_term f_russ_term g_russ_term Eq_russ_term s).
+Qed.
+
+Ltac auto_unfold := repeat
+                     unfold VarInstance_russ_term, Var, ids, Ren_russ_term,
+                      Ren1, ren1, Up_russ_term_russ_term, Up_russ_term,
+                      up_russ_term, Subst_russ_term, Subst1, subst1,
+                      VarInstance_term, Var, ids, Ren_ty, Ren1, ren1,
+                      Ren_term, Ren1, ren1, Up_term_term, Up_term, up_term,
+                      Subst_ty, Subst1, subst1, Subst_term, Subst1, subst1.
+
+Tactic Notation "auto_unfold" "in" "*" := repeat
+                                           unfold VarInstance_russ_term, Var,
+                                            ids, Ren_russ_term, Ren1, ren1,
+                                            Up_russ_term_russ_term,
+                                            Up_russ_term, up_russ_term,
+                                            Subst_russ_term, Subst1, subst1,
+                                            VarInstance_term, Var, ids,
+                                            Ren_ty, Ren1, ren1, Ren_term,
+                                            Ren1, ren1, Up_term_term,
+                                            Up_term, up_term, Subst_ty,
+                                            Subst1, subst1, Subst_term,
+                                            Subst1, subst1 in *.
+
+Ltac asimpl' := repeat (first
+                 [ progress setoid_rewrite substSubst_term_pointwise
+                 | progress setoid_rewrite substSubst_term
+                 | progress setoid_rewrite substSubst_ty_pointwise
+                 | progress setoid_rewrite substSubst_ty
+                 | progress setoid_rewrite substRen_term_pointwise
+                 | progress setoid_rewrite substRen_term
+                 | progress setoid_rewrite substRen_ty_pointwise
+                 | progress setoid_rewrite substRen_ty
+                 | progress setoid_rewrite renSubst_term_pointwise
+                 | progress setoid_rewrite renSubst_term
+                 | progress setoid_rewrite renSubst_ty_pointwise
+                 | progress setoid_rewrite renSubst_ty
+                 | progress setoid_rewrite renRen'_term_pointwise
+                 | progress setoid_rewrite renRen_term
+                 | progress setoid_rewrite renRen'_ty_pointwise
+                 | progress setoid_rewrite renRen_ty
+                 | progress setoid_rewrite substSubst_russ_term_pointwise
+                 | progress setoid_rewrite substSubst_russ_term
+                 | progress setoid_rewrite substRen_russ_term_pointwise
+                 | progress setoid_rewrite substRen_russ_term
+                 | progress setoid_rewrite renSubst_russ_term_pointwise
+                 | progress setoid_rewrite renSubst_russ_term
+                 | progress setoid_rewrite renRen'_russ_term_pointwise
+                 | progress setoid_rewrite renRen_russ_term
+                 | progress setoid_rewrite varLRen'_term_pointwise
+                 | progress setoid_rewrite varLRen'_term
+                 | progress setoid_rewrite varL'_term_pointwise
+                 | progress setoid_rewrite varL'_term
+                 | progress setoid_rewrite rinstId'_term_pointwise
+                 | progress setoid_rewrite rinstId'_term
+                 | progress setoid_rewrite rinstId'_ty_pointwise
+                 | progress setoid_rewrite rinstId'_ty
+                 | progress setoid_rewrite instId'_term_pointwise
+                 | progress setoid_rewrite instId'_term
+                 | progress setoid_rewrite instId'_ty_pointwise
+                 | progress setoid_rewrite instId'_ty
+                 | progress setoid_rewrite varLRen'_russ_term_pointwise
+                 | progress setoid_rewrite varLRen'_russ_term
+                 | progress setoid_rewrite varL'_russ_term_pointwise
+                 | progress setoid_rewrite varL'_russ_term
+                 | progress setoid_rewrite rinstId'_russ_term_pointwise
+                 | progress setoid_rewrite rinstId'_russ_term
+                 | progress setoid_rewrite instId'_russ_term_pointwise
+                 | progress setoid_rewrite instId'_russ_term
+                 | progress
+                    unfold up_term_term, upRen_term_term,
+                     up_russ_term_russ_term, upRen_russ_term_russ_term,
+                     up_ren
+                 | progress
+                    cbn[subst_term subst_ty ren_term ren_ty subst_russ_term
+                       ren_russ_term]
+                 | progress fsimpl ]).
+
+Ltac asimpl := check_no_evars;
+                repeat
+                 unfold VarInstance_russ_term, Var, ids, Ren_russ_term, Ren1,
+                  ren1, Up_russ_term_russ_term, Up_russ_term, up_russ_term,
+                  Subst_russ_term, Subst1, subst1, VarInstance_term, Var,
+                  ids, Ren_ty, Ren1, ren1, Ren_term, Ren1, ren1,
+                  Up_term_term, Up_term, up_term, Subst_ty, Subst1, subst1,
+                  Subst_term, Subst1, subst1 in *; asimpl'; minimize.
+
+Tactic Notation "asimpl" "in" hyp(J) := revert J; asimpl; intros J.
+
+Tactic Notation "auto_case" := auto_case ltac:(asimpl; cbn; eauto).
+
+Ltac substify := auto_unfold; try setoid_rewrite rinstInst'_term_pointwise;
+                  try setoid_rewrite rinstInst'_term;
+                  try setoid_rewrite rinstInst'_ty_pointwise;
+                  try setoid_rewrite rinstInst'_ty;
+                  try setoid_rewrite rinstInst'_russ_term_pointwise;
+                  try setoid_rewrite rinstInst'_russ_term.
+
+Ltac renamify := auto_unfold;
+                  try setoid_rewrite_left rinstInst'_term_pointwise;
+                  try setoid_rewrite_left rinstInst'_term;
+                  try setoid_rewrite_left rinstInst'_ty_pointwise;
+                  try setoid_rewrite_left rinstInst'_ty;
+                  try setoid_rewrite_left rinstInst'_russ_term_pointwise;
+                  try setoid_rewrite_left rinstInst'_russ_term.
+
+End Core.
+
+Module Extra.
+
+Import Core.
+
+#[global] Hint Opaque subst_term: rewrite.
+
+#[global] Hint Opaque subst_ty: rewrite.
+
+#[global] Hint Opaque ren_term: rewrite.
+
+#[global] Hint Opaque ren_ty: rewrite.
+
+#[global] Hint Opaque subst_russ_term: rewrite.
+
+#[global]
+Hint Opaque ren_russ_term: rewrite.
+
+End Extra.
+
+Module interface.
+
+Export Core.
+
+Export Extra.
+
+End interface.
+
+Export interface.
+
